<rdf:RDF
    xmlns:dct="http://purl.org/dc/terms/"
    xmlns:rdf="http://www.w3.org/1999/02/22-rdf-syntax-ns#"
    xmlns:dc="http://purl.org/dc/elements/1.1/"
    xmlns:owl="http://www.w3.org/2002/07/owl#"
    xmlns:skos="http://www.w3.org/2004/02/skos/core#"
    xmlns:rdfs="http://www.w3.org/2000/01/rdf-schema#"
    xmlns:cc="http://creativecommons.org/ns#"
    xmlns:vann="http://purl.org/vocab/vann/">
  <owl:Class rdf:about="https://d-nb.info/standards/vocab/gnd/gender#GenderValue">
    <owl:equivalentClass>
      <owl:Restriction>
        <owl:hasValue>
          <skos:ConceptScheme rdf:about="https://d-nb.info/standards/vocab/gnd/gender#">
            <dc:title xml:lang="de">GND-Geschlecht</dc:title>
            <vann:preferredNamespaceUri>https://d-nb.info/standards/vocab/gnd/gender#</vann:preferredNamespaceUri>
            <dct:modified rdf:datatype="http://www.w3.org/2001/XMLSchema#dateTime"
            >2019-06-13T10:30:00+02:00</dct:modified>
            <owl:priorVersion rdf:resource="http://d-nb.info/standards/vocab/gnd/gender2017-09-12"/>
            <dct:available rdf:datatype="http://www.w3.org/2001/XMLSchema#date"
            >2019-10-15</dct:available>
            <owl:versionIRI rdf:resource="https://d-nb.info/standards/vocab/gnd/gender_20191015"/>
            <owl:versionInfo>1.2</owl:versionInfo>
            <rdfs:comment xml:lang="en">
			Changes from 2017-09-12 to 2019-10-15
			All d-nb.info-URIs changed from http to https
		</rdfs:comment>
            <owl:imports rdf:resource="http://www.w3.org/2004/02/skos/core#"/>
            <dct:rights>Copyright 2012-2019 Deutsche Nationalbibliothek</dct:rights>
            <dc:description xml:lang="en">GND Gender is a value vocabulary (skos:ConceptScheme) listing 
		the possible gender values used in the RDF encoding of the information in the Integrated
		Authority File (Gemeinsame Normdatei, GND).</dc:description>
            <dct:license rdf:resource="http://creativecommons.org/publicdomain/zero/1.0/"/>
            <dct:creator rdf:resource="file:///home/svensson/teamcity/TeamCity/buildAgent/work/661528de212fd35b/src/main/resources/rdf/standards/vocab/gnd/gender.rdf#alexanderHaffner"/>
            <cc:license rdf:resource="http://creativecommons.org/publicdomain/zero/1.0/"/>
            <dct:publisher rdf:resource="http://ld.zdb-services.de/resource/organisations/DE-101"/>
            <rdf:type rdf:resource="http://www.w3.org/2002/07/owl#Ontology"/>
            <dct:issued rdf:datatype="http://www.w3.org/2001/XMLSchema#date"
            >2012-06-30</dct:issued>
            <dc:description xml:lang="de">GND-Geschlecht ist ein RDF value vocabulary (skos:ConceptScheme),
		das die möglichen Werte auflistet, die Geschlechtsangaben in der RDF-Ausgabe der Gemeinsamen
		Normdatei (GND) haben können.</dc:description>
            <vann:preferredNamespacePrefix>gnd-gender</vann:preferredNamespacePrefix>
            <dc:title xml:lang="en">GND Gender</dc:title>
          </skos:ConceptScheme>
        </owl:hasValue>
        <owl:onProperty rdf:resource="http://www.w3.org/2004/02/skos/core#inScheme"/>
      </owl:Restriction>
    </owl:equivalentClass>
    <rdfs:subClassOf rdf:resource="http://www.w3.org/2004/02/skos/core#Concept"/>
    <rdfs:comment xml:lang="de">Die möglichen Instanzen dieser Klasse sind beschränkt auf diejenigen
            skos:Concepts, die zum Concept Scheme &lt;https://d-nb.info/standards/vocab/gnd/gender#&gt; gehören.</rdfs:comment>
    <rdfs:comment xml:lang="en">The possible members of this class is restricted to those skos:Concepts
            that are in the Concept Scheme &lt;https://d-nb.info/standards/vocab/gnd/gender#&gt;.</rdfs:comment>
    <rdfs:label xml:lang="de">Werte für Geschlechtsangabe</rdfs:label>
    <rdfs:label xml:lang="en">Gender Value</rdfs:label>
  </owl:Class>
  <skos:Concept rdf:about="https://d-nb.info/standards/vocab/gnd/gender#male">
    <skos:exactMatch rdf:resource="http://purl.org/linked-data/sdmx/2009/code#sex-M"/>
    <skos:prefLabel xml:lang="en">Male</skos:prefLabel>
    <skos:prefLabel xml:lang="de">Männlich</skos:prefLabel>
    <skos:exactMatch rdf:resource="http://rdvocab.info/termList/gender/1002"/>
    <skos:inScheme rdf:resource="https://d-nb.info/standards/vocab/gnd/gender#"/>
  </skos:Concept>
  <skos:Concept rdf:about="https://d-nb.info/standards/vocab/gnd/gender#notKnown">
    <skos:exactMatch rdf:resource="http://purl.org/linked-data/sdmx/2009/code#sex-U"/>
    <skos:prefLabel xml:lang="en">Not known</skos:prefLabel>
    <skos:prefLabel xml:lang="de">Unbekannt</skos:prefLabel>
    <skos:exactMatch rdf:resource="http://rdvocab.info/termList/gender/1003"/>
    <skos:inScheme rdf:resource="https://d-nb.info/standards/vocab/gnd/gender#"/>
  </skos:Concept>
  <skos:Concept rdf:about="https://d-nb.info/standards/vocab/gnd/gender#female">
    <skos:exactMatch rdf:resource="http://purl.org/linked-data/sdmx/2009/code#sex-F"/>
    <skos:prefLabel xml:lang="en">Female</skos:prefLabel>
    <skos:prefLabel xml:lang="de">Weiblich</skos:prefLabel>
    <skos:exactMatch rdf:resource="http://rdvocab.info/termList/gender/1001"/>
    <skos:inScheme rdf:resource="https://d-nb.info/standards/vocab/gnd/gender#"/>
  </skos:Concept>
</rdf:RDF>
